PropositionalLogic/WeakClassicalPropositionalLogic.v
@@ -1,0 +1,138 @@
+Require Import Coq.Logic.Classical_Prop.
+Require Import Logic.lib.Coqlib.
+Require Import Logic.LogicBase.
+Require Import Logic.MinimunLogic.MinimunLogic.
+Require Import Logic.MinimunLogic.ContextProperty.
+Require Import Logic.PropositionalLogic.Syntax.
+Require Import Logic.PropositionalLogic.IntuitionisticPropositionalLogic.
+
+Local Open Scope logic_base.
+Local Open Scope PropositionalLogic.
+
+Class WeakClassicalPropositionalLogic (L: Language) {nL: NormalLanguage L} {pL: PropositionalLanguage L} (Gamma: ProofTheory L) {mpGamma: MinimunPropositionalLogic L Gamma} {ipGamma: IntuitionisticPropositionalLogic L Gamma} := {
+  impp_choice: forall x y, |-- (x --> y) || (y --> x)
+}.
+
+Lemma derivable_impp_choice: forall {L: Language} {nL: NormalLanguage L} {pL: PropositionalLanguage L} {Gamma: ProofTheory L} {nGamma: NormalProofTheory L Gamma} {mpGamma: MinimunPropositionalLogic L Gamma} {ipGamma: IntuitionisticPropositionalLogic L Gamma} {wpGamma: WeakClassicalPropositionalLogic L Gamma} (Phi: context) (x y: expr),
+  Phi |-- (x --> y) || (y --> x).
+Proof.
+  intros.
+  pose proof impp_choice x.
+  apply deduction_weaken0; auto.
+Qed.
+
+Lemma derivable_weak_excluded_middle: forall {L: Language} {nL: NormalLanguage L} {pL: PropositionalLanguage L} {Gamma: ProofTheory L} {nGamma: NormalProofTheory L Gamma} {mpGamma: MinimunPropositionalLogic L Gamma} {ipGamma: IntuitionisticPropositionalLogic L Gamma} {wpGamma: WeakClassicalPropositionalLogic L Gamma} (Phi: context) (x: expr),
+  Phi |-- ~~ x || ~~ ~~ x.
+Proof.
+  intros.
+  pose proof derivable_impp_choice Phi x (~~ x).
+  
+  assert (Phi |-- (x --> ~~ x) --> (x --> FF)).
+  Focus 1. {
+    rewrite <- deduction_theorem.
+    rewrite <- deduction_theorem.
+    eapply deduction_weaken with (Union _ (Union _ (Union _ Phi (Singleton _ (x --> ~~ x))) (Singleton _ x)) (Singleton _ x)).
+    + intros y ?.
+      destruct H0; [| right; auto].
+      destruct H0; [| right; auto].
+      left; auto.
+    + rewrite deduction_theorem.
+      rewrite deduction_theorem.
+      apply derivable_assum1.
+  } Unfocus.
+  assert (Phi |-- (~~ x --> x) --> (~~ x --> FF)).
+  Focus 1. {
+    rewrite <- deduction_theorem.
+    pose proof derivable_assum1 Phi (~~ x --> x).
+    set (Psi := Union expr Phi (Singleton expr (~~ x --> x))) in H1 |- *; clearbody Psi.
+    rewrite <- deduction_theorem in H1 |- *.
+    pose proof derivable_assum1 Psi (~~ x).
+    pose proof deduction_modus_ponens _ _ _ H1 H2.
+    auto.
+  } Unfocus.
+
+  rewrite <- deduction_theorem in H0, H1.
+  apply (deduction_orp_intros1 _ _ (~~ x --> FF)) in H0.
+  apply (deduction_orp_intros2 _ (x --> FF)) in H1.
+  rewrite deduction_theorem in H0, H1.
+  pose proof deduction_orp_elim _ _ _ _ H0 H1.
+  pose proof deduction_modus_ponens _ _ _ H H2.
+  auto.
+Qed.
+(*
+Lemma DCS_negp_iff: forall {L: Language} {nL: NormalLanguage L} {pL: PropositionalLanguage L} {Gamma: ProofTheory L} {nGamma: NormalProofTheory L Gamma} {mpGamma: MinimunPropositionalLogic L Gamma} {ipGamma: IntuitionisticPropositionalLogic L Gamma} {cpGamma: ClassicalPropositionalLogic L Gamma} (Phi: context),
+  derivable_closed Phi ->
+  orp_witnessed Phi ->
+  consistent Phi ->
+  (forall x: expr, Phi x <-> ~ Phi (~~ x)).
+Proof.
+  intros.
+  split; intros.
+  + rewrite derivable_closed_element_derivable in H2 |- * by auto.
+    intro.
+    pose proof deduction_modus_ponens _ _ _ H2 H3.
+    rewrite consistent_spec in H1; apply H1; auto.
+  + rewrite derivable_closed_element_derivable in H2 |- * by auto.
+    pose proof derivable_excluded_middle Phi x.
+    specialize (H0 x (~~ x)).
+    rewrite derivable_closed_element_derivable in H0 by auto.
+    apply H0 in H3.
+    destruct H3; rewrite derivable_closed_element_derivable in H3 by auto; auto.
+    tauto.
+Qed.
+*)
+Module WeakClassicalPropositionalLogic.
+Section WeakClassicalPropositionalLogic.
+
+Context (Var: Type).
+
+Instance L: Language := PropositionalLanguage.L Var.
+Instance nL: NormalLanguage L := PropositionalLanguage.nL Var.
+Instance pL: PropositionalLanguage L := PropositionalLanguage.pL Var.
+
+Inductive provable: expr -> Prop :=
+| modus_ponens: forall x y, provable (x --> y) -> provable x -> provable y
+| axiom1: forall x y, provable (x --> (y --> x))
+| axiom2: forall x y z, provable ((x --> y --> z) --> (x --> y) --> (x --> z))
+| andp_intros: forall x y, provable (x --> y --> x && y)
+| andp_elim1: forall x y, provable (x && y --> x)
+| andp_elim2: forall x y, provable (x && y --> y)
+| orp_intros1: forall x y, provable (x --> x || y)
+| orp_intros2: forall x y, provable (y --> x || y)
+| orp_elim: forall x y z, provable ((x --> z) --> (y --> z) --> (x || y --> z))
+| falsep_elim: forall x, provable (FF --> x)
+| impp_choice: forall x y, provable ((x --> y) || (y --> x)).
+
+Instance G: ProofTheory L := Build_AxiomaticProofTheory provable.
+
+Instance nG: NormalProofTheory L G := Build_nAxiomaticProofTheory provable.
+
+Instance mpG: MinimunPropositionalLogic L G.
+Proof.
+  constructor.
+  + apply modus_ponens.
+  + apply axiom1.
+  + apply axiom2.
+Qed.
+
+Instance ipG: IntuitionisticPropositionalLogic L G.
+Proof.
+  constructor.
+  + apply andp_intros.
+  + apply andp_elim1.
+  + apply andp_elim2.
+  + apply orp_intros1.
+  + apply orp_intros2.
+  + apply orp_elim.
+  + apply falsep_elim.
+Qed.
+
+Instance wpG: WeakClassicalPropositionalLogic L G.
+Proof.
+  constructor.
+  apply impp_choice.
+Qed.
+
+End WeakClassicalPropositionalLogic.
+End WeakClassicalPropositionalLogic.
+
