Makefile
@@ -9,6 +9,7 @@ all: Wf.vo base.vo IPC.vo trivial.vo Kripke.vo enumerate.vo LogicBase.vo \
      PropositionalLogic/IntuitionisticPropositionalLogic.vo \
      PropositionalLogic/KripkeSemantics.vo \
      PropositionalLogic/Syntax.vo PropositionalLogic/ClassicalPropositionalLogic.vo \
+     PropositionalLogic/WeakClassicalPropositionalLogic.vo \
      PropositionalLogic/TrivialSemantics.vo PropositionalLogic/Sound_Classical_Trivial.vo \
      PropositionalLogic/Complete_Classical_Trivial.vo lib/Coqlib.vo \
      lib/Bijection.vo lib/Countable.vo PropositionalLogic/Complete_Intuitionistic_Kripke.vo \
